Updated SmallVec dependency interface

proofs/fstar/dependencies/Smallvec.fst
@@ -3,7 +3,71 @@ module Smallvec
 open Core
 open FStar.Mul
 
-assume
-val t_SmallVec': v_T: Type0 -> v_N: usize -> eqtype
+/// Types that can be used as the backing store for a [`SmallVec`].
+class t_SmallVecArray (v_Self: Type0) = {
+  f_Item:Type0;
+  f_size_pre:Prims.unit -> Type0;
+  f_size_post:Prims.unit -> usize -> Type0;
+  f_size:x0: Prims.unit -> Prims.Pure usize (f_size_pre x0) (fun result -> f_size_post x0 result)
+}
 
-let t_SmallVec (v_T: Type0) (v_N: usize) = t_SmallVec' v_T v_N
+assume
+val t_SmallVecData': v_A: Type0 -> {| i1: t_SmallVecArray v_A |} -> eqtype
+
+let t_SmallVecData (v_A: Type0) (#[FStar.Tactics.Typeclasses.tcresolve ()] i1: t_SmallVecArray v_A) =
+  t_SmallVecData' v_A #i1
+
+/// A `Vec`-like container that can store a small number of elements inline.
+/// `SmallVec` acts like a vector, but can store a limited amount of data inline within the
+/// `SmallVec` struct rather than in a separate allocation.  If the data exceeds this limit, the
+/// `SmallVec` will "spill" its data onto the heap, allocating a new buffer to hold it.
+/// The amount of data that a `SmallVec` can store inline depends on its backing store. The backing
+/// store can be any type that implements the `Array` trait; usually it is a small fixed-sized
+/// array.  For example a `SmallVec<[u64; 8]>` can hold up to eight 64-bit integers inline.
+/// ## Example
+/// ```rust
+/// use smallvec::SmallVec;
+/// let mut v = SmallVec::<[u8; 4]>::new(); // initialize an empty vector
+/// // The vector can hold up to 4 items without spilling onto the heap.
+/// v.extend(0..4);
+/// assert_eq!(v.len(), 4);
+/// assert!(!v.spilled());
+/// // Pushing another element will force the buffer to spill:
+/// v.push(4);
+/// assert_eq!(v.len(), 5);
+/// assert!(v.spilled());
+/// ```
+type t_SmallVec (v_A: Type0) {| i1: t_SmallVecArray v_A |} = {
+  f_capacity:usize;
+  f_data:t_SmallVecData v_A
+}
+
+/// Creates a `SmallVec` with `n` copies of `elem`.
+/// ```
+/// use smallvec::SmallVec;
+/// let v = SmallVec::<[char; 128]>::from_elem(\'d\', 2);
+/// assert_eq!(v, SmallVec::from_buf([\'d\', \'d\']));
+/// ```
+assume
+val impl_17__from_elem':
+    #v_A: Type0 ->
+    {| i1: t_SmallVecArray v_A |} ->
+    {| i2: Core.Clone.t_Clone i1.f_Item |} ->
+    elem: i1.f_Item ->
+    n: usize
+  -> t_SmallVec v_A
+
+let impl_17__from_elem
+      (#v_A: Type0)
+      (#[FStar.Tactics.Typeclasses.tcresolve ()] i1: t_SmallVecArray v_A)
+      (#[FStar.Tactics.Typeclasses.tcresolve ()] i2: Core.Clone.t_Clone i1.f_Item)
+     = impl_17__from_elem' #v_A #i1 #i2
+
+[@@ FStar.Tactics.Typeclasses.tcinstance]
+let impl_61 (#v_T: Type0) : t_SmallVecArray (t_Array v_T (mk_usize 2)) =
+  {
+    f_Item = v_T;
+    f_size_pre = (fun (_: Prims.unit) -> true);
+    f_size_post = (fun (_: Prims.unit) (out: usize) -> true);
+    f_size = fun (_: Prims.unit) -> mk_usize 2
+  }
